Jian helped!
\begin{enumerate}
	\item[(a)] \begin{align*}
		 \text{The stabilized system is }\begin{cases}
		 	\dot q &= v \\
		 	m\,\dot v &= f - G^T\,\lambda \\
		 	0 &= \ddot g + \gamma_1\,\dot g + \gamma_2\,g \\		 	
		 \end{cases}
		\end{align*}
	\fbox{\begin{minipage}[h!]{\textwidth}
			$\gamma_1$ and $\gamma_2$ chosen such that the root of the polynomial $s^2 + s\,\gamma_1 + \gamma_2 = 0$ is located in the left-half of the complex plane. 
	\end{minipage}}	
	\item[(b)] \begin{align*}
		\text{Original system: }\begin{cases}
			\dot q &= v \\
			M\,\dot v &= f - G^T\,\lambda \\
			0 &= G\,v = h\\		 	
		\end{cases}
	\end{align*}
	$\dot h + \gamma\,h = 0$ is the stabilization, equivalent to, $G\,\dot v + \frac{\partial G\,v}{\partial q}\,v + \gamma\,G\,v = 0$.
	Therefore, we get:
	\begin{align*}
		\begin{cases}
			\dot q = v \quad & e_1 \\
			M\,\dot v = f - G^T\,\lambda \quad & e_2\\
			G\,\dot v + \frac{\partial G\,v}{\partial q}\,v + \gamma\,G\,v = 0 \quad & e_1\\		 	
		\end{cases}
	\end{align*}
	Focusing on $e_2$:
	Multiply both sides with $G\,M^{-1}$, we get:
	\begin{align*}
		G\,\dot v &= G\,M^{-1}\,f - G\,M^{-1}\,G^T\,\lambda & e_2,\\
		\implies -\frac{\partial G\,v}{\partial q}\,v + \gamma\,G\,v &= G\,M^{-1}\,f - G\,M^{-1}\,G^T\,\lambda & e_2.
	\end{align*}
	Therefore,
	\begin{align*}
		\lambda&= \left(G\,M^{-1}\,G^T\right)^{-1}\,\left(G\,M^{-1}\,f + \frac{\partial G\,v}{\partial q}\,v + \gamma\,G\,v\right)& e_3
	\end{align*}
	substituting $e_3$ in $e_2$, we get:
	\begin{align*}
		\dot v &= M^{-1}\,f - M^{-1}\,G^T\,\left(G\,M^{-1}\,G^T\right)^{-1}\,\left(G\,M^{-1}\,f + \frac{\partial G\,v}{\partial q}\,v + \gamma\,G\,v\right)& e_4
	\end{align*}
	The system equations are:
	\begin{align*}
		\begin{cases}
			\dot q = v \quad & e_1 \\
			\dot v = M^{-1}\,f - M^{-1}\,G^T\,\left(G\,M^{-1}\,G^T\right)^{-1}\,\left(G\,M^{-1}\,f + \frac{\partial G\,v}{\partial q}\,v + \gamma\,G\,v\right) \quad &  e_4 	
		\end{cases}
	\end{align*}
	This is equivalent to:
	\begin{align*}
		\begin{pmatrix}
			\dot q \\
			\dot v 
		\end{pmatrix} &= \hat f(x) - \gamma\,F(x)\,h(x)
	\end{align*}
\end{enumerate}