Jian helped! 

The index 3 DAE is given as follows:
\begin{align*}
	x &= g(t) & \implies x &= g\\
	\dot x - y &= 0 & \implies y &= \dot g\\
	\dot y - z &= 0 & \implies z &= \ddot g\\
\end{align*}
Assuming that $\frac{h_{n-1}}{h_n}$ is not $\infty$, then $\mathcal{O}(h_{n}\,h_{n-1}) = \mathcal{O}(h_n^2)$. 

From the DAE system we have:
\begin{align*}
	y_n &= \frac{g_n - g_{n-1}}{h_n},\\
	y_{n-1} &= \frac{g_{n-1} - g_{n-2}}{h_{n-1}},\\
	z_n &= \frac{y_n - y_{n-1}}{h_n},\\
\end{align*}
Now, 
\begin{align*}
	g_{n-1} &= g_n - \dot g_n\,h_n + \frac{1}{2}\,h_n^2\,\ddot g_n + \mathcal{O}(h_n^3),\\
	g_{n-2} &= g_n - \dot g_n\,\left(h_n + h_{n-1}\right) + \frac{1}{2}\,\left(h_n + h_{n-1}\right)^2\,\ddot g_n + \mathcal{O}(h_n^3)
\end{align*}
Thus, 
\begin{align*}
	z_n &= \frac{y_n - y_{n-1}}{h_n} = \frac{\frac{g_n - g_{n-1}}{h_n} - \frac{g_{n-1} - g_{n-2}}{h_{n-1}}}{h_n} =  \frac{1}{2}\,\left(1+\frac{h_{n-1}}{h_n}\right)\,\ddot g + \mathcal{O}(h_n)
\end{align*}
The error is,
\begin{align*}
	z_n - \ddot g_n = \frac{1}{2}\,\left(\frac{h_{n-1}}{h_n} - 1 \right)\,\ddot g + \mathcal{O}(h_n)
\end{align*}
